coo summation

COO.v
@@ -6,6 +6,7 @@ Hint Rewrite conseq_cons' : rew_listx.
 
 Open Scope Z_scope.
 
+
 Definition to_int (v : val) : int := 
   match v with 
   | val_int i => i 
@@ -28,9 +29,33 @@ Lemma NoDup_nthZ {A : Type} i j l (z : A):
   (0<= j < Datatypes.length l) -> nth (abs i) l z = nth (abs j) l z -> i = j).
 Admitted.
 
+Lemma in_combineE {A B : Type} (l : list A) (l' : list B) (x : A) (y : B) :
+  In (x, y) (combine l l') = (In x l /\ In y l').
+Admitted.
+
 End pure_facts.
 
 Module coo_vec.
+
+Module Export AD := WithUnary(IntDom).
+
+Lemma hbig_fset_part {A : Type} (fs : fset A) (P : A -> Prop) : 
+  hbig_fset hstar fs = 
+  fun H => hbig_fset hstar (fs ∩ P) H \* hbig_fset hstar (fs ∖ P) H.
+Proof.
+  apply/fun_ext_1=> ?; rewrite -hbig_fset_union // ?fs_pred_part //.
+  exact/fs_pred_part_disj.
+Qed.
+
+Notation "H1 '\\*' H2" := (hstar H1 H2)
+  (at level 42, right associativity, format "H1  \\* '//' H2") : hprop_scope.
+
+
+Notation "'for' i <- '[' Z ',' N ']' '{' t '}'"  :=
+  (For Z N <{ fun_ i => t }>)
+  (in custom trm at level 69,
+    Z, N, i at level 0,
+    format "'[' for  i  <-  [ Z ','  N ] ']'  '{' '/   ' '[' t  '}' ']'") : trm_scope.
 
 Section coo_vec.
 
@@ -88,20 +113,6 @@ Proof.
   xapp; xsimpl*; rewrite memNindex // nth_overflow //; math.
 Qed.
 
-(* Lemma htriple_union_pointwise (fs : fset D) (H : D -> hhprop) (Q : D -> (D -> val) -> hhprop) ht 
-  (Hcong : forall d hv1 hv2, hv1 d = hv2 d -> Q d hv1 ==> Q d hv2) :
-  forall (Htp : forall d, indom fs d -> htriple (single d tt) ht (H d) (Q d)),
-  htriple fs ht (\*_(d <- fs) H d) (fun hv => \*_(d <- fs) (Q d hv)).
-Proof. *)
-
-Lemma hbig_fset_part {A : Type} (fs : fset A) (P : A -> Prop) : 
-  hbig_fset hstar fs = 
-  fun H => hbig_fset hstar (fs ∩ P) H \* hbig_fset hstar (fs ∖ P) H.
-Proof.
-  apply/fun_ext_1=> ?; rewrite -hbig_fset_union // ?fs_pred_part //.
-  exact/fs_pred_part_disj.
-Qed.
-
 
 Lemma get_spec_out `{Inhab D} fs (x_ind x_val : loc) : 
   htriple  fs
@@ -122,11 +133,6 @@ Proof.
   xsimpl*.
 Qed.
 
-Notation "'for' i <- '[' Z ',' N ']' '{' t '}'"  :=
-  (For Z N <{ fun_ i => t }>)
-  (in custom trm at level 69,
-    Z, N, i at level 0,
-    format "'[' for  i  <-  [ Z ','  N ] ']'  '{' '/   ' '[' t  '}' ']'") : trm_scope.
 
 Definition sum := 
   <{
@@ -138,11 +144,6 @@ Definition sum :=
   };
   ! s
 }>.
-
-Print HD.type.
-
-Notation "H1 '\\*' H2" := (hstar H1 H2)
-  (at level 42, right associativity, format "H1  \\* '//' H2") : hprop_scope.
 
 (* Tactic Notation "xin" constr(S1) ":" tactic(tac) := 
   let n := constr:(S1) in
@@ -176,7 +177,7 @@ Proof with fold'.
   have E : `[0,M] ∩ xind = xind.
   { apply/fset_extens=> x; rewrite /intr filter_indom -fset_of_list_in; splits*.
     move=> ?; splits*; rewrite* indom_interval. }
-  rewrite E fset_of_list_nodup // len_xind.
+  rewrite E (fset_of_list_nodup 0) // len_xind.
   set (R i := arr(x_ind, xind)⟨2, i⟩ \* arr(x_val, xval)⟨2, i⟩).
   set (Inv (i : int) := arr(x_ind, xind)⟨1, 0⟩ \* arr(x_val, xval)⟨1, 0⟩).
   xfor_sum Inv R (fun=> \Top) (fun hv i => hv[`2](xind[i])) s.
@@ -187,9 +188,9 @@ Proof with fold'.
     move/NoDup_nthZ: nodup_xind; apply; autos*; math. }
   { rewrite -len_xind; math. }
   xapp; xsimpl.
-  under (@SumEq _ _ `[0,M]).
+  under (@SumEq _ _ _ `[0,M]).
   { move=>*; rewrite to_int_if; over. }
-  rewrite SumIf E SumList // len_xind Sum0s; math.
+  rewrite SumIf E (SumList 0) // len_xind Sum0s; math.
 Qed.
 
 Context (dvec : list int).
@@ -208,8 +209,6 @@ Definition dotprod :=
   };
   ! s
 }>.
-
-Opaque harray_int.
 
 Lemma SumIf {A : Type} {P : A -> Prop} {fs F G} (C : A -> int -> int) : 
   (Σ_(i <- fs) C i (If P i then F i else G i)) = 
@@ -242,7 +241,7 @@ Proof with fold'.
   have E : `[0,M] ∩ xind = xind.
   { apply/fset_extens=> x; rewrite /intr filter_indom -fset_of_list_in; splits*.
     move=> ?; splits*; rewrite* indom_interval. }
-  rewrite E fset_of_list_nodup // len_xind.
+  rewrite E (fset_of_list_nodup 0) // len_xind.
   set (R i := arr(x_ind, xind)⟨2, i⟩ \* arr(x_val, xval)⟨2, i⟩ \* arr(d_vec, dvec)⟨2,i⟩).
   set (Inv (i : int) := arr(x_ind, xind)⟨1, 0⟩ \* arr(x_val, xval)⟨1, 0⟩ \* arr(d_vec, dvec)⟨1,0⟩).
   xfor_sum Inv R (fun=> \Top) (fun hv i => (hv[`2](xind[i]) * dvec[xind[i] ])) s.
@@ -253,14 +252,204 @@ Proof with fold'.
     move/NoDup_nthZ: nodup_xind; apply; autos*; math. }
   { rewrite -len_xind; math. }
   xapp; xsimpl.
-  under (@SumEq _ _ `[0,M]).
+  under (@SumEq _ _ _ `[0,M]).
   { move=>*; rewrite to_int_if; over. }
-  rewrite (SumIf (fun=> Z.mul^~ _)) E SumList // len_xind Sum0s; math.
+  rewrite (SumIf (fun=> Z.mul^~ _)) E (SumList 0) // len_xind Sum0s; math.
 Qed.
 
 End coo_vec.
 
 
 End coo_vec.
+
+
+
+Module coo. 
+
+Module Export AD2 := WithUnary(Int2Dom).
+
+Lemma hbig_fset_part {A : Type} (fs : fset A) (P : A -> Prop) : 
+  hbig_fset hstar fs = 
+  fun H => hbig_fset hstar (fs ∩ P) H \* hbig_fset hstar (fs ∖ P) H.
+Proof.
+  apply/fun_ext_1=> ?; rewrite -hbig_fset_union // ?fs_pred_part //.
+  exact/fs_pred_part_disj.
+Qed.
+
+Notation "H1 '\\*' H2" := (hstar H1 H2)
+  (at level 42, right associativity, format "H1  \\* '//' H2") : hprop_scope.
+
+
+Notation "'for' i <- '[' Z ',' N ']' '{' t '}'"  :=
+  (For Z N <{ fun_ i => t }>)
+  (in custom trm at level 69,
+    Z, N, i at level 0,
+    format "'[' for  i  <-  [ Z ','  N ] ']'  '{' '/   ' '[' t  '}' ']'") : trm_scope.
+
+Section coo.
+
+Notation "'dvec'" := ("d_vec":var) (in custom trm at level 0) : trm_scope.
+Notation "'xrow'" := ("x_row":var) (in custom trm at level 0) : trm_scope.
+Notation "'xcol'" := ("x_col":var) (in custom trm at level 0) : trm_scope.
+Notation "'xval'" := ("x_val":var) (in custom trm at level 0) : trm_scope.
+
+Import List Vars.
+
+Context (xrow xcol xval : list int).
+Context (N Nrow Ncol : int).
+Hypothesis len_xrow : length xrow = N :> int.
+Hypothesis len_xcol : length xcol = N :> int.
+Hypothesis len_xval : length xval = N :> int.
+Hypothesis nodup_xrowcol : NoDup (combine xrow xcol).
+Hypothesis xrow_leq : forall x, In x xrow -> 0 <= x < Nrow.
+Hypothesis xcol_leq : forall x, In x xcol -> 0 <= x < Ncol.
+
+Definition indexf := index2.func N.
+
+Definition get := 
+  <{
+  fun i j xrow xcol xval =>
+    let k = indexf i j xrow xcol in 
+    read_array xval k
+}>.
+
+Lemma get_spec_in `{Inhab D} (x_row x_col x_val : loc) i d : 
+  htriple (single d tt) 
+    (fun=> get (List.nth (abs i) xrow 0) (List.nth (abs i) xcol 0) x_row x_col x_val)
+    (\[0 <= i < N] \*
+      harray_int xrow x_row d \* 
+      harray_int xcol x_col d \* 
+      harray_int xval x_val d)
+    (fun hr => 
+     \[hr = fun=> List.nth (abs i) xval 0] \* 
+      harray_int xrow x_row d \* 
+      harray_int xcol x_col d \* 
+      harray_int xval x_val d).
+Proof.
+  rewrite -wp_equiv; xsimpl=> ?.
+  xwp; xapp index2.spec=> //.
+  xapp; xsimpl*; rewrite -combine_nth; last lia. 
+  rewrite index_nodup // combine_length; lia. 
+Qed.
+
+Lemma get_spec_out_unary `{Inhab D} (x_row x_col x_val : loc) (i j : int) d : 
+  htriple (single d tt) 
+    (fun=> get i j x_row x_col x_val)
+    (\[~ In (i, j) (combine xrow xcol)] \*
+      harray_int xrow x_row d \* 
+      harray_int xcol x_col d \* 
+      harray_int xval x_val d)
+    (fun hr => 
+     \[hr = fun=> 0] \* 
+      harray_int xrow x_row d \* 
+      harray_int xcol x_col d \* 
+      harray_int xval x_val d).
+Proof.
+  rewrite -wp_equiv; xsimpl=> ?.
+  xwp; xapp index2.spec=> //.
+  xapp; xsimpl*; rewrite memNindex // nth_overflow // combine_length; lia.
+Qed.
+
+Lemma get_spec_out `{Inhab D} fs (x_row x_col x_val : loc) : 
+  htriple fs
+    (fun i => get (eld i).1 (eld i).2 x_row x_col x_val)
+    (\[forall d, indom fs d -> ~ In (eld d) (combine xrow xcol)] \*
+      (\*_(d <- fs) harray_int xrow x_row d) \* 
+      (\*_(d <- fs) harray_int xcol x_col d) \* 
+       \*_(d <- fs) harray_int xval x_val d)
+    (fun hr => 
+     \[hr = fun=> 0] \* 
+      (\*_(d <- fs) harray_int xrow x_row d) \*
+      (\*_(d <- fs) harray_int xcol x_col d) \*  
+       \*_(d <- fs) harray_int xval x_val d).
+Proof.
+  apply/htriple_val_eq/htriple_conseq;
+  [|eauto|move=> ?]; rewrite -hstar_fset_pure -?hbig_fset_hstar; first last.
+  { move=> ?; apply: applys_eq_init; reflexivity. }
+  apply/htriple_union_pointwise=> [> -> //|[?][??]?]. 
+  rewrite -wp_equiv wp_single. 
+  xapp get_spec_out_unary=> //= ??->.
+  xsimpl*.
+Qed.
+
+(* Lemma SumIf {A : Type} {P : A -> Prop} {fs F G} (C : A -> int -> int) : 
+  (Σ_(i <- fs) C i (If P i then F i else G i)) = 
+  Σ_(i <- fs ∩ P) C i (F i) + Σ_(i <- fs ∖ P) C i (G i).
+Proof using.
+Admitted. *)
+
+Definition sum := 
+  <{
+  fun xval =>
+  let s = ref 0 in
+  for i <- [0, N] {
+    let x = xval[i] in 
+    s += x
+  };
+  ! s
+}>.
+
+Ltac fold' := 
+  rewrite ?label_single ?wp_single
+    (* -/(incr _)  *)
+    -/(For_aux _ _) 
+    -/(For _ _ _) //=.
+
+
+Lemma sum_spec `{Inhab D} (x_row x_col x_val : loc) : 
+  {{ arr(x_row, xrow)⟨1, (0,0)⟩ \\*
+     arr(x_col, xcol)⟨1, (0,0)⟩ \\*
+     arr(x_val, xval)⟨1, (0,0)⟩ \\*
+     (\*_(i <- `[0, Nrow] \x `[0, Ncol]) arr(x_row, xrow)⟨2, i⟩) \\*
+     (\*_(i <- `[0, Nrow] \x `[0, Ncol]) arr(x_col, xcol)⟨2, i⟩) \\*
+     (\*_(i <- `[0, Nrow] \x `[0, Ncol]) arr(x_val, xval)⟨2, i⟩) }}
+  [{
+    [1| ld in `{(0,0)}   => sum x_val];
+    {2| ld in `[0, Nrow] \x `[0, Ncol] => get ld.1 ld.2 x_row x_col x_val}
+  }]
+  {{ hv, \[hv[`1]((0,0)) = Σ_(i <- `[0, Nrow] \x `[0, Ncol]) hv[`2](i)] \* \Top}}.
+Proof with fold'.
+  have lE: length (combine xrow xcol) = N :> int by rewrite combine_length; lia.
+  xfocus (2,0) (combine xrow xcol).
+  rewrite (hbig_fset_part (`[0, Nrow] \x `[0, Ncol]) (combine xrow xcol)). (* TODO: move to xfocus *)
+  xapp get_spec_out=> //.
+  { case=> ?? /[! @indom_label_eq]-[_]/=. 
+    rewrite /intr filter_indom indom_prod; autos*. }
+  set (H1 := hbig_fset hstar (_ ∖ _) _); 
+  set (H2 := hbig_fset hstar (_ ∖ _) _);
+  set (H3 := hbig_fset hstar (_ ∖ _) _).
+  xframe (H1 \* H2 \* H3); clear H1 H2 H3.
+  xin (1,0) : xwp; xapp=> s...
+  have E : (`[0, Nrow] \x `[0, Ncol]) ∩ combine xrow xcol = combine xrow xcol.
+  { apply/fset_extens=> -[??]. 
+    rewrite /intr filter_indom indom_prod -fset_of_list_in; splits*.
+    rewrite /Sum.mem in_combineE /= ?indom_interval=> -[]; autos*. }
+  rewrite ?E (fset_of_list_nodup (0,0)) // lE.
+  set (R i := 
+    arr(x_row, xrow)⟨2, i⟩ \*
+    arr(x_col, xcol)⟨2, i⟩ \* 
+    arr(x_val, xval)⟨2, i⟩).
+  set (Inv (i : int) := 
+    arr(x_row, xrow)⟨1, (0,0)⟩ \* 
+    arr(x_col, xcol)⟨1, (0,0)⟩ \* 
+    arr(x_val, xval)⟨1, (0,0)⟩).
+  xfor_sum Inv R (fun=> \Top) (fun hv i => hv[`2]((xrow[i], xcol[i]))) s.
+  { rewrite /Inv /R.
+    (xin (1,0): (xwp; xapp; xapp incr.spec=> y))...
+    rewrite ?combine_nth /=; try lia.
+    xapp get_spec_in=> //; xsimpl*. }
+  { move=> Neq ???; apply/Neq. 
+    move/NoDup_nthZ: nodup_xrowcol; apply; autos*; math. }
+  { rewrite combine_nth //; lia. }
+  { lia. }
+  xapp; xsimpl.
+  under (@SumEq _ _ _ (`[0, Nrow] \x `[0, Ncol])).
+  { move=>*; rewrite to_int_if; over. }
+  rewrite SumIf E. (SumList 0). // len_xind Sum0s; math.
+Qed.
+
+End coo.
+
+End coo.
 
 
